WIP

Multistep.v
@@ -8,32 +8,39 @@ From Elo Require Import TypeProperties.
 (* ------------------------------------------------------------------------- *)
 
 Definition invariants m ths :=
-  forall_memory  m      value              /\
-  forall_program m ths (valid_term m)      /\
-  no_uninitialized_references m ths        /\
-  unique_initializers         m ths        /\
-  unique_critical_regions     m ths        /\
-  forall_program m ths well_typed_term     /\
-  forall_program m ths (consistent_term m) /\
-  memory_pointer_types m                   /\
-  forall_program m ths safe_term           /\
-  init_cr_exclusivity  ths                 /\
-  forall_memory_consistent_regions  m      /\
-  forall_threads_consistent_regions m ths   .
+  forall_memory  m      value                     /\
+  forall_program m ths  keywords                  /\
+  forall_program m ths (valid_term m)             /\
+  forall_program m ths (consistent_waits WR_none) /\
+  no_uninitialized_references m ths               /\
+  unique_initializers         m ths               /\
+  unique_holding              m ths               /\
+  forall_program m ths well_typed_term            /\
+  forall_program m ths (consistent_term m)        /\
+  memory_pointer_types m                          /\
+  forall_program m ths safe_term                  /\
+  init_cr_exclusivity  ths                        /\
+  forall_memory_consistent_regions  m             /\
+  forall_threads_consistent_regions m ths          .
 
 Theorem invariants_preservation_base : forall t,
-  no_refs         t ->
-  no_inits        t ->
-  no_crs          t ->
-  well_typed_term t ->
+  no_refs t                  ->
+  no_inits t                 ->
+  no_crs t                   ->
+  no_reacqs t                ->
+  keywords t                 ->
+  consistent_waits WR_none t ->
+  well_typed_term t          ->
   invariants nil (base t).
 Proof.
   intros.
   split; eauto using forallmemory_base.
+  split; eauto using kw_preservation_base.
   split; eauto using vtm_preservation_base.
+  split; eauto using cw_preservation_base.
   split; eauto using nur_preservation_base.
   split; eauto using ui_preservation_base.
-  split; eauto using ucr_preservation_base.
+  split; eauto using uhg_preservation_base.
   split; eauto using wtt_preservation_base.
   split; eauto using ctm_preservation_base.
   split; eauto using mpt_preservation_base.
@@ -41,26 +48,6 @@ Proof.
   split; eauto using ice_preservation_base.
   split; eauto using mcreg_preservation_base.
          eauto using creg_preservation_base.
-Qed.
-
-Theorem invariants_preservation_rstep : forall m1 m2 ths1 ths2 tid e,
-  invariants m1 ths1 ->
-  m1 \ ths1 ~~~[tid, e]~~> m2 \ ths2 ->
-  invariants m2 ths2.
-Proof.
-  intros * H ?. unfold invariants in *. decompose record H. clear H.
-  split; eauto using value_preservation_rstep.
-  split; eauto using vtm_preservation_rstep.
-  split; eauto using nur_preservation_rstep.
-  split; eauto using ui_preservation_rstep.
-  split; eauto using ucr_preservation_rstep.
-  split; eauto using wtt_preservation_rstep.
-  split; eauto using ctm_preservation_rstep.
-  split; eauto using mpt_preservation_rstep.
-  split; eauto using stm_preservation_rstep.
-  split; eauto using ice_preservation_rstep.
-  split; eauto using mcreg_preservation_rstep.
-         eauto using creg_preservation_rstep.
 Qed.
 
 Theorem invariants_preservation_ustep : forall m1 m2 ths1 ths2 tc,
@@ -71,29 +58,33 @@ Proof.
   intros * H ?. ind_ustep; trivial.
   spec. unfold invariants in *. decompose record IHmultistep. clear IHmultistep.
   assert (forall_memory m3 value)
-    by eauto using value_preservation_rstep.
+    by eauto using value_preservation_cstep.
+  assert (forall_program m3 ths3 keywords)
+    by eauto using kw_preservation_cstep.
   assert (forall_program m3 ths3 (valid_term m3))
-    by eauto using vtm_preservation_rstep.
+    by eauto using vtm_preservation_cstep.
+  assert (forall_program m3 ths3 (consistent_waits WR_none))
+    by eauto using cw_preservation_cstep .
   assert (no_uninitialized_references m3 ths3)
-    by eauto using nur_preservation_rstep.
+    by eauto using nur_preservation_cstep.
   assert (unique_initializers m3 ths3)
-    by eauto using ui_preservation_rstep.
-  assert (unique_critical_regions m3 ths3)
-    by eauto using ucr_preservation_rstep.
+    by eauto using ui_preservation_cstep.
+  assert (unique_holding m3 ths3)
+    by eauto using uhg_preservation_cstep.
   assert (forall_program m3 ths3 well_typed_term)
-    by eauto using wtt_preservation_rstep.
+    by eauto using wtt_preservation_cstep.
   assert (forall_program m3 ths3 (consistent_term m3))
-    by eauto using ctm_preservation_rstep.
+    by eauto using ctm_preservation_cstep.
   assert (memory_pointer_types m3)
-    by eauto using mpt_preservation_rstep.
+    by eauto using mpt_preservation_cstep.
   assert (forall_program m3 ths3 safe_term)
-    by eauto using stm_preservation_rstep.
+    by eauto using stm_preservation_cstep.
   assert (init_cr_exclusivity ths3)
-    by eauto using ice_preservation_rstep.
+    by eauto using ice_preservation_cstep.
   assert (forall_memory_consistent_regions m3)
-    by eauto using mcreg_preservation_rstep.
+    by eauto using mcreg_preservation_cstep.
   assert (forall_threads_consistent_regions m3 ths3)
-    by eauto using creg_preservation_rstep.
+    by eauto using creg_preservation_cstep.
   repeat (split; trivial).
 Qed.
 
@@ -121,8 +112,16 @@ Corollary des_inva_value : forall m ths,
   invariants m ths -> forall_memory m value.
 Proof. solve_inva_des. Qed.
 
+Corollary des_inva_kw : forall m ths,
+  invariants m ths -> forall_program m ths keywords.
+Proof. solve_inva_des. Qed.
+
 Corollary des_inva_vtm : forall m ths,
   invariants m ths -> forall_program m ths (valid_term m).
+Proof. solve_inva_des. Qed.
+
+Corollary des_inva_cw : forall m ths,
+  invariants m ths -> forall_program m ths (consistent_waits WR_none).
 Proof. solve_inva_des. Qed.
 
 Corollary des_inva_nur : forall m ths,
@@ -133,8 +132,8 @@ Corollary des_inva_ui : forall m ths,
   invariants m ths -> unique_initializers m ths.
 Proof. solve_inva_des. Qed.
 
-Corollary des_inva_ucr : forall m ths,
-  invariants m ths -> unique_critical_regions m ths.
+Corollary des_inva_mu : forall m ths,
+  invariants m ths -> unique_holding m ths.
 Proof. solve_inva_des. Qed.
 
 Corollary des_inva_wtt : forall m ths,
@@ -173,10 +172,12 @@ Proof. solve_inva_des. Qed.
   des_forallprogram_memory
   des_forallprogram_threads
   des_inva_value
+  des_inva_kw
   des_inva_vtm
+  des_inva_cw
   des_inva_nur
   des_inva_ui
-  des_inva_ucr
+  des_inva_mu
   des_inva_wtt
   des_inva_ctm
   des_inva_mpt
